Intermediate/Typing.lean
@@ -1,0 +1,24 @@
+import Intermediate.Global
+import Core.Ty
+import Surface.Term
+
+import Lilac
+open Lilac
+
+namespace Intermediate
+
+
+inductive VecTyping (J : A -> B -> Prop) : Vec A m -> Vec B m -> Prop
+| nil : VecTyping J .nil .nil
+| cons :
+  J a b ->
+  VecTyping J as bs ->
+  VecTyping J (a::as) (b::bs)
+
+def Query (G : List Global) (c : DataConst) (qs : Vec String m) (Ts : Vec Core.Ty m) : Prop :=
+  VecTyping (lookup_ctor? G c · ·) qs Ts
+
+def Query.Match (qs : Vec String m) (ps : Core.Pattern m) : Prop :=
+  VecTyping (λ q p => ∃ na As nb, p = ⟨q, na, As, nb⟩) qs ps
+
+end Intermediate
